specs/Spec.Chacha20.fst
@@ -1,6 +1,5 @@
 module Spec.Chacha20
 
-
 open FStar.Mul
 open Lib.IntTypes
 open Lib.Sequence
